\documentclass{article}
\usepackage[utf8]{inputenc}
\usepackage{amsmath}
\usepackage{geometry}[margins=1in]

\title{Induction}
\author{smgrmd }
\date{May 2019}

\begin{document}

\section{Problem}
Show that for composition of finitely many invertible functions is invertible.

\section{Solution}
This proof can be performed with induction.
The base case consists of a single invertible function.
By definition, such a function is invertible. \\

Suppose that this holds true for a function composed of $k$ invertible functions is itself invertible. \\
$g(x) = (f_k \circ \ldots \circ f_1)(x) \Rightarrow \exists h(x) : (h \circ g)(x) = 1$ \\
Then in order to complete the proof by induction, we must demonstrate that a function composed of $k+1$ invertible functions is invertible. \\

Consider $i(x) = (f_{k+1} \circ g)(x)$.
We know that for $\forall f_{k+1}(x) \exists f_{k+1}^{-1}(x): (f_{k+1}^{-1} \circ f_{k+1})(x) = 1$.
Let $j(x) = (h \circ f_{k+1}^{-1})(x)$.
Then $(j \circ i)(x) = ((h \circ f_{k+1}^{-1}) \circ (f_{k+1} \circ g))(x) = (h \circ (f_{k+1}^{-1} \circ f_{k+1}) \circ g)(x) = (h \circ g)(x) = 1$.
This demonstrates that a function composed of $k+1$ invertible functions is invertible.
Consequently, we complete our proof by induction.

\end{document}

